\documentclass[journal,12pt,twocolumn]{IEEEtran}
\usepackage{enumitem}
\usepackage{amsmath}
\usepackage{amssymb}
\usepackage{gensymb}
\usepackage{graphicx}
\usepackage{txfonts}         
\usepackage{listings}
\usepackage{lstautogobble}
\usepackage{mathtools}
\usepackage{bm}
\usepackage{hyperref}
\usepackage{polynom}
\usepackage{capt-of}
\usepackage{circuitikz}
\newcommand{\solution}{\noindent \textbf{Solution: }}
\providecommand{\pr}[1]{\ensuremath{\Pr\left(#1\right)}}
\providecommand{\brak}[1]{\ensuremath{\left(#1\right)}}
\providecommand{\cbrak}[1]{\ensuremath{\left\{#1\right\}}}
\providecommand{\sbrak}[1]{\ensuremath{\left[#1\right]}}
\providecommand{\mean}[1]{E\left[ #1 \right]}
\providecommand{\var}[1]{\mathrm{Var}\left[ #1 \right]}
\providecommand{\der}[1]{\mathrm{d} #1}
\providecommand{\gauss}[2]{\mathcal{N}\ensuremath{\left(#1,#2\right)}}
\providecommand{\mbf}{\mathbf}
\providecommand{\abs}[1]{\left\vert#1\right\vert}
\providecommand{\norm}[1]{\left\lVert#1\right\rVert}
\providecommand{\z}[1]{{\mathcal{Z}}\{#1\}}
\providecommand{\ztrans}{\overset{\mathcal{Z}}{ \rightleftharpoons}}
\providecommand{\system}[1]{\overset{\mathcal{#1}}{ \longleftrightarrow}}
\providecommand{\laplaceinv}[1]{{\mathcal{L}^{-1}\ensuremath{\left[#1\right]}}}
\providecommand{\parder}[2]{\frac{\partial}{\partial #2} \brak{#1}}

\let\StandardTheFigure\thefigure
\let\vec\mathbf

\numberwithin{equation}{section}
\renewcommand{\thefigure}{\theenumi}
\renewcommand\thesection{\arabic{section}}

\newcommand{\myvec}[1]{\ensuremath{\begin{pmatrix}#1\end{pmatrix}}}
\newcommand{\mydet}[1]{\ensuremath{\begin{vmatrix}#1\end{vmatrix}}}
\newcommand{\define}{\stackrel{\triangle}{=}}

\DeclareMathOperator*{\argmin}{arg\,min}
\DeclareMathOperator*{\argmax}{arg\,max}


\lstset {
	frame=single, 
	breaklines=true,
	columns=fullflexible,
	autogobble=true
}             
   


\begin{document}
                             
\title{ Digital Signal Processing \\ Circuits and Transforms}
\author{Suraj Kumar\\ \normalsize AI21BTECH11029}
 \maketitle 
 \tableofcontents
 \section{Definitions}
\begin{enumerate}[label=\arabic*.,ref=\thesection.\theenumi]
\numberwithin{equation}{section}
\numberwithin{figure}{section}
\item The unit step function is 
\begin{align}
\label{eq:unit-step}
u(t) =
\begin{cases}
1 & t > 0
\\
	\frac{1}{2} & t = 0
\\
0 & t < 0
\end{cases}
\end{align}
\item The Laplace transform of $g(t)$ is defined as 
\begin{align}
	G(s) = \int_{-\infty}^{\infty} g(t) e^{-st}\, dt
\end{align}
 \end{enumerate}

 \section{Laplace Transform}
\begin{enumerate}[label=\arabic*.,ref=\thesection.\theenumi]
\numberwithin{equation}{section}
\item In the circuit, the switch S is connected to position P for a long time so that the charge on the capacitor
	becomes $q_1 \, \mu C$. Then S is switched to position Q.  After a long time, the charge on the capacitor is
		$q_2 \, \mu C$.
		\begin{figure}[!ht]
			\centering
			\includegraphics[width=\columnwidth]{figs/ckt.jpg}
			\caption{}
			\label{fig:ckt}
\end{figure}
\item Draw the circuit using latex-tikz.\\
\solution The following code yields Fig.\ref{fig:qn}
\begin{lstlisting}
wget https://raw.githubusercontent.com/kumarsuraj151/EE3900/master/cktsig/Tikz%20Circuits/2_2.tex
\end{lstlisting}
\begin{figure}[!ht]
 \centering
  \input{Tikz Circuits/2_2.tex}
\caption{Given Circuit}
\label{fig:qn}
\end{figure}

\item Find $q_1$.\\
\solution
Before switching S to Q:
Calculating current,
\begin{align}
1-i-2i-2=0\\
3i=-1 \Rightarrow i=\frac{-1}{3}
\end{align}
\begin{figure}
	\centering
	 \input{Tikz Circuits/2_3.tex}
   \caption{Before switching S to Q}
   \label{fig:c1}
\end{figure}
Potential Difference between capacitor at steady state is
\begin{align}
1-\brak{\frac{-1}{3}}=\frac{4}{3}\\
q_1=\frac{4}{3} \cdot 1\\
=\frac{4}{3} \mu C
\end{align}
	\item Show that the Laplace transform of $u(t)$ is $\frac{1}{s}$ and find the ROC.\\
	\solution We know that from definition of Laplace Transform,
	\begin{align}
	\label{eq:lap-tran}
	F(s)&= \int_{0}^{\infty} f(t)e^{-st} \,dt 
	\end{align}
	for $u(t)$, we have
	\begin{align}
		U(s)&=\int_{0}^{\infty} u(t)e^{-st} \,dt
	\end{align}
	Using \eqref{eq:unit-step},
	\begin{align}
	U(s)&=\int_{0}^{\infty} u(t)e^{-st} \,dt\\
	&=\int_{0}^{\infty} e^{-st} \,dt\\
	&=-\brak{0-\frac{1}{s}}\\
	&=\frac{1}{s}
	\end{align}
	ROC is $ Re(s)>0$ since $e^{-st}<\infty$ for $t \to \infty$
	The following command plots the ROC of above Laplace Transform.
	\begin{lstlisting}
wget  https://raw.githubusercontent.com/kumarsuraj151/EE3900/master/cktsig/code/2_4.py	
\end{lstlisting}
	\begin{figure}[!ht]
			\centering
			\includegraphics[width=\columnwidth]{figs/2.4.png}
			\caption{}
			\label{fig:roc1}
\end{figure}

\item Show that 
		\begin{align}
			e^{-at}u(t) \system{L} \frac{1}{s+a}, \quad a > 0
		\end{align}
		and find the ROC.
		\solution From \eqref{eq:lap-tran},
		\begin{align}
		F(s)&=\int_{0}^{\infty} u(t)e^{-at}e^{-st} \,dt\\
		&=\int_{0}^{\infty} u(t)e^{-\brak{s+a}t} \,dt\\
		&=\int_{0}^{\infty} e^{-\brak{s+a}t} \,dt\\
		&=-\brak{0-\frac{1}{s+a}}\\
		&=\frac{1}{s+a}
		\end{align}
		ROC is
		\begin{align}
		s+a>0 \Rightarrow s>-a
		\end{align}
		The following command plots the ROC of above Laplace Transform.
	\begin{lstlisting}
wget  https://raw.githubusercontent.com/kumarsuraj151/EE3900/master/cktsig/code/2_5.py	
\end{lstlisting}
		\begin{figure}[!ht]
			\centering
			\includegraphics[width=\columnwidth]{figs/2.5.png}
			\caption{}
			\label{fig:roc2}
\end{figure}
	\item Now consider the following resistive circuit transformed from 
			Fig. \ref{fig:ckt}
		\begin{figure}[!ht]
			\centering
			\includegraphics[width=\columnwidth]{figs/lap-ckt.jpg}
			\caption{}
			\label{fig:lap-ckt}
\end{figure}
		where 
		\begin{align}
			u(t) \system{L} V_1(s)
			\\
			2u(t) \system{L} V_2(s)
		\end{align}
		Find the voltage across the capacitor $V_{C_0}(s)$.
		\solution
		\begin{align}
		R_{eff}=\frac{1}{1+\frac{1}{2}}
		=\frac{2}{3} \Omega\\
		V_{eff}=\frac{1}{1+\frac{1}{2}}
		=\frac{2}{3} V
		\end{align}
		%Effective Circuit in Laplacian Space is
	
\begin{align}
V_{C_0}(s)&=V_{S}(s)\frac{C_{0}}{C_{0}+R_{eff}}\\
&=\brak{\frac{4}{3s}}\brak{\frac{\frac{1}{s}}{\frac{1}{s}+\frac23}}\\
\label{eq:laptr}
&=\frac{6}{s\brak{4s+9}}
\end{align}
	\item Find $v_{C_0}(t)$.  Plot using python.\\
	\solution Using \eqref{eq:laptr},
	\begin{align}
	\frac{6}{s\brak{4s+9}}&=\frac{4}{3s}-\frac{2}{9+4s}
	\end{align}
	Apply inverse Laplacian Transform,
	\begin{align}
	V_{C_0}(s)\system{L^{-1}}V_{C_0}(t)\\
	\laplaceinv{V_{C_0}(s)}&=\laplaceinv{\frac{4}{3s}-\frac{2}{9+4s}}\\
&=	\laplaceinv{\frac{4}{3s}}-\laplaceinv{\frac{2}{9+4s}}
\end{align}
Since,
\begin{align}
\laplaceinv{\frac1s}&=u(t)\\
\laplaceinv{\frac{1}{s-a}}&=e^{at}u(t)
\end{align}
Using the above equations,
\begin{align}
V_{C_0}(t)=\frac{4}{3}\brak{ 1-e^{\frac{-3}{2} t}}u(t)
	\end{align}
	The following command plots the above equation.
	\begin{lstlisting}
wget  https://raw.githubusercontent.com/kumarsuraj151/EE3900/master/cktsig/code/2_7.py		
\end{lstlisting}
	\begin{figure}[!ht]
			\centering
			\includegraphics[width=\columnwidth]{figs/2.7.png}
			\caption{Plot of $V_{C_0}(t)$}
			\label{fig:lap-ckt}
\end{figure}
	\item Verify your result using ngspice.\\
	\solution The following command plots the ROC of above Laplace Transform.
	\begin{lstlisting}
wget  https://raw.githubusercontent.com/kumarsuraj151/EE3900/master/cktsig/code/2_8.cir
\end{lstlisting}
\begin{figure}[!ht]
			\centering
			\includegraphics[width=\columnwidth]{figs/2.8.png}
			\caption{}
			\label{fig:ckt}
\end{figure}
\end{enumerate}

 \section{Initial Conditions}
\begin{enumerate}[label=\arabic*.,ref=\thesection.\theenumi]
\numberwithin{equation}{section}
\item Find $q_2$ in Fig. 
			\ref{fig:ckt}.\\
			\solution At steady state, $V_{C_0}=V_{1 \Omega}$
			\begin{align*}
			V_{C_0}=\frac{q_2}{C}=V_{1 \Omega}=\frac{2}{1+2}=\frac23\\
			q_2=\frac23 \mu C
			\end{align*}
\item Draw the equivalent $s$-domain resistive circuit when S is switched to position Q.  Use variables $R_1, R_2, C_0$ for the passive elements.
Use latex-tikz.
		\label{prob:init}\\
		\solution 
		The following command plots the ROC of above Laplace Transform.
	\begin{lstlisting}
wget https://raw.githubusercontent.com/kumarsuraj151/EE3900/master/cktsig/Tikz%20Circuits/3_2.tex
\end{lstlisting}
	\begin{figure}[!ht]
 \centering
\input{Tikz Circuits/3_2.tex}
\caption{After switching S to Q}
\label{fig:sq}
\end{figure}
		\item $V_{C_0}(s)$ = ? \\
		\solution Using KCL at node in Fig. \ref{fig:sq}
\begin{align}
    \frac{V - 0}{R_1} + \frac{V - \frac{2}{s}}{R_2} + sC_0\brak{V - \frac{4}{3s}} = 0 \\
\implies V_{C_0}(s) = \frac{\frac{2}{sR_2} + \frac{4C_0}{3}}{\frac{1}{R_1} + \frac{2}{R_2} + sC_0}
\label{eq:v2-s}
\end{align} 
	\item $v_{C_0}(t)$ = ? Plot using python.\\
	\solution From \eqref{eq:v2-s},
\begin{align}
    &V_{C_0}(s) = \frac{4}{3}\brak{\frac{1}{\frac{1}{C_0}\brak{\frac{1}{R_1} + \frac{1}{R_2}}+s}} \nonumber \\
    &+ \frac{2}{R_2\brak{\frac{1}{R_1} +\frac{1}{R_2}}}\brak{\frac{1}{s} - \frac{1}{\frac{1}{C_0}\brak{\frac{1}{R_1} + \frac{1}{R_2}} + s}}
\end{align}
Taking an inverse Laplace Transform,
\begin{align}
    &v_{C_0}(t) = \frac{4}{3}e^{-\brak{\frac{1}{R_1} + \frac{1}{R_2}}\frac{t}{C_0}}u(t) \nonumber \\ 
    &+ \frac{2}{R_2\brak{\frac{1}{R_1}+\frac{1}{R_2}}}\brak{1 - e^{-\brak{\frac{1}{R_1} + \frac{1}{R_2}}\frac{t}{C_0}}}u(t)
\end{align}
Substituting values gives
\begin{align}
    v_{C_0}(t) = \frac{2}{3}\brak{1 +e^{-\brak{1.5 \times 10^6}t}}u(t)
    \label{eq:v2-t}
\end{align}
The following command plots the above equation.
	\begin{lscolumnwidthtlisting}
wget https://raw.githubusercontent.com/kumarsuraj151/EE3900/master/cktsig/code/3_4.py
\end{lstlisting}
\begin{figure}[!ht]
			\centering
			\includegraphics[width=\columnwidth]{figs/3.4}
			\caption{Plot of $V_{C_0}(t)$}
			\label{fig:lap-ckt}
\end{figure}
	\item Verify your result using ngspice.\\
	\solution The following command plots Fig.3.3
	\begin{lstlisting}
wget https://raw.githubusercontent.com/kumarsuraj151/EE3900/master/cktsig/code/3.5.cir
\end{lstlisting}
	 \begin{figure}[!ht]
			\centering
			\includegraphics[width=\columnwidth]{figs/3.5}
			% \caption{}
			% \label{fig:ckt}
\end{figure}
	\item Find $v_{C_0}(0-), v_{C_0}(0+)$ and  $v_{C_0}(\infty) $. 

\solution From the initial conditions,
\begin{align}
    v_{C_0}(0-) = \frac{q_1}{C} = {\frac{4}{3}}{V}
\end{align}
Using \eqref{eq:v2-t},
\begin{align}
    v_{C_0}(0+) &= \lim_{t \to 0+}v_{C_0}(t) = {\frac{4}{3}}{V} \\
    v_{C_0}(\infty) &= \lim_{t \to \infty}v_{C_0}(t) = {\frac{2}{3}}{V}
\end{align}

\item Obtain Fig. \ref{prob:init} using the equivalent differential equation
	
	\solution Using Kirchoff's junction law
	\begin{align}
		\frac{v_c(t) - 0}{R_1} + \frac{v_c(t) - v_2(t)}{R_2} + \frac{\der{q}}{\der{t}} = 0
	\end{align}
	where $q(t)$ is the charge on the capacitor
	
	On taking the Laplace transform on both sides of this equation
	\begin{align}
		\frac{V_c(s) - 0}{R_1} + \frac{V_c(s) - V_2(s)}{R_2} + \brak{sQ(s) - q(0^-)} = 0
	\end{align}
	
	But $q(0^-) = \frac43 C_0$ and 
	\begin{align}
		q(t) &= C_0v_c(t) \\
		\implies Q(s) &= C_0V_c(s)
	\end{align}
	
	Thus
	\begin{align}
		&\frac{V_c(s) - 0}{R_1} + \frac{V_c(s) - V_2(s)}{R_2} + \brak{sC_0V_c(s) - \frac43 C_0} = 0 \\
		\implies &\frac{V_c(s) - 0}{R_1} + 	\frac{V_c(s) - V_2(s)}{R_2} + \frac{V_c(s) - \frac{4}{3s}}{\frac{1}{sC_0}} = 0 
	\end{align}
	
	which is the same equation as the one we obtained from Fig. \ref{prob:init}
	\end{enumerate}

 \section{Bilinear Transform}
\begin{enumerate}[label=\arabic*.,ref=\thesection.\theenumi]
\numberwithin{equation}{section}
\item In Fig. 
			\ref{fig:ckt},
			consider the case when $S$ is switched to $Q$ right in the beginning. Formulate the differential equation.\\
	\solution The differential equation is the same as before 
	\begin{align}
		&\frac{v_c(t) - 0}{R_1} + \frac{v_c(t) - v_2(t)}{R_2} + \frac{\der{q}}{\der{t}} = 0 \\
		\text{i.e., } &\frac{v_c(t)}{R_1} + \frac{v_c(t) - v_2(t)}{R_2} + C_0\frac{\der{v_c}}{\der{t}} = 0
	\end{align}
	\begin{equation}
		q(0^-) = q(0) = 0
	\end{equation}
\item 			Find $H(s)$ considering the ouput voltage at the capacitor.\\
\solution On taking the Laplace transform on both sides of this equation
\begin{align}
	&\frac{V_c(s)}{R_1} + \frac{V_c(s) - V_2(s)}{R_2} + sQ(s) - 0 = 0 \\
	\implies &V_c(s) \brak{\frac{1}{R_1} + \frac{1}{R_2}} + sC_0V_c(s) = \frac{V_2(s)}{R_2} \\
	\implies &\frac{V_c(s)}{V_2(s)} = \frac{\frac{1}{R_2}}{\frac{1}{R_1} + \frac{1}{R_2} + sC_0}
\end{align}
\begin{align}
	H(s)=\frac{V_c(s)}{V_2(s)} = \frac{\frac{1}{R_2C_0}}{s + \frac{1}{R_1C_0} + \frac{1}{R_2C_0}}\\
	H(s) = \frac{5 \times 10^5}{s + 1.5 \times 10^6}
\end{align}
\item Plot $H(s)$.  What kind of filter is it?
\solution Download the following Python code that plots Fig. \ref{fig-4.3}
	\begin{lstlisting}
		wget https://raw.githubusercontent.com/kumarsuraj151/EE3900/master/cktsig/Tikz%20Circuits/4.3.tex
	\end{lstlisting}
	\begin{figure}[!ht]
		\centering
		\includegraphics[width=\columnwidth]{./figs/4.3}
		\caption{Plot of $H(s)$}
		\label{fig-4.3}	
	\end{figure}
	\begin{align}
		H(\j\omega) &= \frac{5 \times 10^5}{\j\omega + 1.5 \times 10^6} \\
		\implies \abs{H(\j\omega)} &= \frac{5 \times 10^5}{\sqrt{\omega^2 + 2.25\times10^{12}}}
	\end{align}
	
	As $\omega$ increases, $\abs{H(\j\omega)}$ decreases.
	
	In other words, the amplitude of high-frequency signals gets diminished and they get filtered out.
	
	Therefore, this is a low-pass filter.
		\item Using trapezoidal rule for integration, formulate the difference equation
			by considering 
		\begin{align}
			y(n) = y(t)\vert_{t=n}
		\end{align}
	\solution
\begin{align}
	&\frac{v_c(t)}{R_1} + \frac{v_c(t) - v_2(t)}{R_2} + C_0\frac{\der{v_c}}{\der{t}} = 0 \\
	\implies &C_0\frac{\der{v_c}}{\der{t}} = \frac{2u(t)-v_c(t)}{R_2} - \frac{v_c(t)}{R_1} \\
	\implies &\left.v_c(t)\right|_{t=n}^{n+1} = \int_{n}^{n+1} \brak{\frac{2u(t)-v_c(t)}{R_2C_0} - \frac{v_c(t)}{R_1C_0}} \der{t}
\end{align}

By the trapezoidal rule of integration
\begin{align}
	\int_a^b f(t) \der{t} \approx \frac{b-a}{2} (f(a) + f(b))
\end{align}

Consider $y(t) = v_c(t)$
\begin{multline}
	y(n+1) - y(n) = \frac{1}{R_2C_0}\brak{u(n)+u(n+1)} \\
	- \frac12(y(n+1) + y(n))\brak{\frac{1}{R_1C_0} + \frac{1}{R_2C_0}}
\end{multline}

Thus, the difference equation is
\begin{multline}
	y(n+1) \brak{1 + \frac{1}{2R_1C_0} + \frac{1}{2R_2C_0}} \\= y(n) \brak{1 - \frac{1}{2R_1C_0} - \frac{1}{2R_2C_0}} \\+ \frac{1}{R_2C_0}\brak{u(n)+u(n+1)}
	\end{multline}
	\item Find $H(z)$.\\
	 \solution Let $\z{y(n)} = Y(z)$
	
	On taking the $Z$-transform on both sides of the difference equation
	\begin{multline}
		zY(z)\brak{1 + \frac{1}{2R_1C_0} + \frac{1}{2R_2C_0}} \\= Y(z)\brak{1 - \frac{1}{2R_1C_0} - \frac{1}{2R_2C_0}} \\+ \frac{1}{R_2C_0} \brak{\frac{1}{1-z^{-1}} + \frac{z}{1-z^{-1}}}
	\end{multline}
	\begin{multline}
		Y(z)\brak{z + \frac{z}{2R_1C_0} + \frac{z}{2R_2C_0} - 1 + \frac{1}{2R_1C_0} + \frac{1}{2R_2C_0}} \\
		= \frac{1}{R_2C_0} \frac{1+z}{1-z^{-1}}
	\end{multline}
	
	Also
	\begin{align}
		v_2(t) &= 2 &&\forall t \ge 0\\
		\implies x(n) &= 2u(n) \\
		\implies X(z) &= \frac{2}{1-z^{-1}} &&\abs{z} > 1
	\end{align}
	
	Thus, the transfer function in $z$-domain is
	\begin{align}
		H(z) &= \frac{Y(z)}{X(z)} \\
		&= \frac{\frac{1+z}{2R_2C_0}}{z + \frac{z}{2R_1C_0} + \frac{z}{2R_2C_0} - 1 + \frac{1}{2R_1C_0} + \frac{1}{2R_2C_0}} \\
		&= \frac{\frac{1 + z^{-1}}{2R_2C_0}}{1 + \frac{1}{2R_1C_0} + \frac{1}{2R_2C_0} - z^{-1} + \frac{z^{-1}}{2R_1C_0} + \frac{z^{-1}}{2R_2C_0}}
	\end{align}
	
	On substituting the values
	\begin{align}
		H(z) &= \frac{2.5\times10^5 (1+z^{-1})}{7.5\times10^5 + 1 + (7.5\times10^5 - 1)z^{-1}}
	\end{align}
	
	with the ROC being
	\begin{align}
		\abs{z} &> \max\brak{1, \abs{\frac{7.5\times10^5 - 1}{7.5\times10^5 + 1}}} \\
		\implies \abs{z} &> 1
	\end{align}
	\item How can you obtain $H(z)$ from $H(s)$?\\f
	\solution The $Z$-transform can be obtained from the Laplace transform by the substitution
	\begin{align}
		s &= \frac{2}{T} \frac{1-z^{-1}}{1+z^{-1}}
	\end{align}
	where $T$ is the step size of the trapezoidal rule ($1$ in our case)
	
	This is known as the bilinear transform
	
	Thus
	\begin{align}
		H(z) &= \frac{\frac{1}{R_2C_0}}{2\frac{1-z^{-1}}{1+z^{-1}} + \frac{1}{R_1C_0} + \frac{1}{R_2C_0}} \\
		&= \frac{\frac{1 + z^{-1}}{2R_2C_0}}{1-z^{-1}	 + \brak{\frac{1}{2R_1C_0} + \frac{1}{2R_2C_0}}(1 + z^{-1})} \\
		&= \frac{\frac{1 + z^{-1}}{2R_2C_0}}{1 + \frac{1}{2R_1C_0} + \frac{1}{2R_2C_0} - z^{-1} + \frac{z^{-1}}{2R_1C_0} + \frac{z^{-1}}{2R_2C_0}} \\
		&= \frac{2.5\times10^5 (1+z^{-1})}{7.5\times10^5 + 1 + (7.5\times10^5 - 1)z^{-1}}
	\end{align}
	which is the same as what we obtained earlier
	\end{enumerate}
\end{document}