\documentclass[journal,12pt,twocolumn]{IEEEtran}
%
\usepackage{setspace}
\usepackage{gensymb}
\usepackage{xcolor}
\usepackage{caption}
%\usepackage{subcaption}
%\doublespacing
\singlespacing

%\usepackage{graphicx}
%\usepackage{amssymb}
%\usepackage{relsize}
\usepackage[cmex10]{amsmath}
\usepackage{mathtools}
%\usepackage{amsthm}
%\interdisplaylinepenalty=2500
%\savesymbol{iint}
%\usepackage{txfonts}
%\restoresymbol{TXF}{iint}
%\usepackage{wasysym}
\usepackage{hyperref}
\usepackage{amsthm}
\usepackage{mathrsfs}
\usepackage{txfonts}
\usepackage{stfloats}
\usepackage{cite}
\usepackage{cases}
\usepackage{subfig}
%\usepackage{xtab}
\usepackage{longtable}
\usepackage{multirow}
%\usepackage{algorithm}
%\usepackage{algpseudocode}
%\usepackage{enumerate}
\usepackage{enumitem}
\usepackage{mathtools}
%\usepackage{iithtlc}
%\usepackage[framemethod=tikz]{mdframed}
\usepackage{listings}
\let\vec\mathbf
\usepackage{tikz}

%\usepackage{stmaryrd}


%\usepackage{wasysym}
%\newcounter{MYtempeqncnt}
\DeclareMathOperator*{\Res}{Res}
%\renewcommand{\baselinestretch}{2}
\renewcommand\thesection{\arabic{section}}
\renewcommand\thesubsection{\thesection.\arabic{subsection}}
\renewcommand\thesubsubsection{\thesubsection.\arabic{subsubsection}}

\renewcommand\thesectiondis{\arabic{section}}
\renewcommand\thesubsectiondis{\thesectiondis.\arabic{subsection}}
\renewcommand\thesubsubsectiondis{\thesubsectiondis.\arabic{subsubsection}}

%\renewcommand{\labelenumi}{\textbf{\theenumi}}
%\renewcommand{\theenumi}{P.\arabic{enumi}}

% correct bad hyphenation here
\hyphenation{op-tical net-works semi-conduc-tor}

\lstset{
language=Python,
frame=single, 
breaklines=true,
columns=fullflexible
}



\begin{document}
%

\theoremstyle{definition}
\newtheorem{theorem}{Theorem}[section]
\newtheorem{problem}{Problem}
\newtheorem{proposition}{Proposition}[section]
\newtheorem{lemma}{Lemma}[section]
\newtheorem{corollary}[theorem]{Corollary}
\newtheorem{example}{Example}[section]
\newtheorem{definition}{Definition}[section]
%\newtheorem{algorithm}{Algorithm}[section]
%\newtheorem{cor}{Corollary}
\newcommand{\BEQA}{\begin{eqnarray}}
\newcommand{\EEQA}{\end{eqnarray}}
\newcommand{\define}{\stackrel{\triangle}{=}}
\newcommand{\myvec}[1]{\ensuremath{\begin{pmatrix}#1\end{pmatrix}}}
\newcommand{\mydet}[1]{\ensuremath{\begin{vmatrix}#1\end{vmatrix}}}

\bibliographystyle{IEEEtran}
%\bibliographystyle{ieeetr}

\providecommand{\nCr}[2]{\,^{#1}C_{#2}} % nCr
\providecommand{\nPr}[2]{\,^{#1}P_{#2}} % nPr
\providecommand{\mbf}{\mathbf}
\providecommand{\pr}[1]{\ensuremath{\Pr\left(#1\right)}}
\providecommand{\qfunc}[1]{\ensuremath{Q\left(#1\right)}}
\providecommand{\sbrak}[1]{\ensuremath{{}\left[#1\right]}}
\providecommand{\lsbrak}[1]{\ensuremath{{}\left[#1\right.}}
\providecommand{\rsbrak}[1]{\ensuremath{{}\left.#1\right]}}
\providecommand{\brak}[1]{\ensuremath{\left(#1\right)}}
\providecommand{\lbrak}[1]{\ensuremath{\left(#1\right.}}
\providecommand{\rbrak}[1]{\ensuremath{\left.#1\right)}}
\providecommand{\cbrak}[1]{\ensuremath{\left\{#1\right\}}}
\providecommand{\lcbrak}[1]{\ensuremath{\left\{#1\right.}}
\providecommand{\rcbrak}[1]{\ensuremath{\left.#1\right\}}}
\providecommand{\rect}[1]{\text{rect}\ensuremath{\left(#1\right)}}
\providecommand{\sinc}[1]{\text{sinc}\ensuremath{\left(#1\right)}}
\theoremstyle{remark}
\newtheorem{rem}{Remark}
\newcommand{\sgn}{\mathop{\mathrm{sgn}}}
\providecommand{\abs}[1]{\left\vert#1\right\vert}
\providecommand{\res}[1]{\Res\displaylimits_{#1}} 
\providecommand{\norm}[1]{\lVert#1\rVert}
\providecommand{\mtx}[1]{\mathbf{#1}}
\providecommand{\mean}[1]{E\left[ #1 \right]}
\providecommand{\fourier}{\overset{\mathcal{F}}{ \rightleftharpoons}}
\providecommand{\ztrans}{\overset{\mathcal{Z}}{ \rightleftharpoons}}
\providecommand{\foutranin}[1]{\mathcal{F}\cbrak{#1}}
\providecommand{\foutranfin}[1]{\int_{-\infty}^{\infty}{#1}e^{-j2\pi ft}\,dt}

%\providecommand{\hilbert}{\overset{\mathcal{H}}{ \rightleftharpoons}}
%\providecommand{\system}{\overset{\mathcal{H}}{ \longleftrightarrow}}
\providecommand{\system}[1]{\overset{\mathcal{#1}}{ \longleftrightarrow}}
	%\newcommand{\solution}[2]{\textbf{Solution:}{#1}}
\newcommand{\solution}{\noindent \textbf{Solution: }}
\providecommand{\dec}[2]{\ensuremath{\overset{#1}{\underset{#2}{\gtrless}}}}
\numberwithin{equation}{section}
%\numberwithin{equation}{subsection}
%\numberwithin{problem}{subsection}
%\numberwithin{definition}{subsection}
\makeatletter
\@addtoreset{figure}{problem}
\makeatother

\let\StandardTheFigure\thefigure
%\renewcommand{\thefigure}{\theproblem.\arabic{figure}}
\renewcommand{\thefigure}{\theproblem}


%\numberwithin{figure}{subsection}

\def\putbox#1#2#3{\makebox[0in][l]{\makebox[#1][l]{}\raisebox{\baselineskip}[0in][0in]{\raisebox{#2}[0in][0in]{#3}}}}
     \def\rightbox#1{\makebox[0in][r]{#1}}
     \def\centbox#1{\makebox[0in]{#1}}
     \def\topbox#1{\raisebox{-\baselineskip}[0in][0in]{#1}}
     \def\midbox#1{\raisebox{-0.5\baselineskip}[0in][0in]{#1}}

\vspace{3cm}

\title{ 
%\logo{
%}
Fourier Series
%	\logo{Octave for Math Computing }
}
%\title{
%	\logo{Matrix Analysis through Octave}{\begin{center}\includegraphics[scale=.24]{tlc}\end{center}}{}{HAMDSP}
%}


% paper title
% can use linebreaks \\ within to get better formatting as desired
%\title{Matrix Analysis through Octave}
%
%
% author names and IEEE memberships
% note positions of commas and nonbreaking spaces ( ~ ) LaTeX will not break
% a structure at a ~ so this keeps an author's name from being broken across
% two lines.
% use \thanks{} to gain access to the first footnote area
% a separate \thanks must be used for each paragraph as LaTeX2e's \thanks
% was not built to handle multiple paragraphs
%

\author{ Suraj kumar\\
AI21BTECH11029% <-this % stops a space
%\thanks{J. Doe and J. Doe are with Anonymous University.}% <-this % stops a space
%\thanks{Manuscript received April 19, 2005; revised January 11, 2007.}}
}
% note the % following the last \IEEEmembership and also \thanks - 
% these prevent an unwanted space from occurring between the last author name
% and the end of the author line. i.e., if you had this:
% 
% \author{....lastname \thanks{...} \thanks{...} }
%                     ^------------^------------^----Do not want these spaces!
%
% a space would be appended to the last name and could cause every name on that
% line to be shifted left slightly. This is one of those "LaTeX things". For
% instance, "\textbf{A} \textbf{B}" will typeset as "A B" not "AB". To get
% "AB" then you have to do: "\textbf{A}\textbf{B}"
% \thanks is no different in this regard, so shield the last } of each \thanks
% that ends a line with a % and do not let a space in before the next \thanks.
% Spaces after \IEEEmembership other than the last one are OK (and needed) as
% you are supposed to have spaces between the names. For what it is worth,
% this is a minor point as most people would not even notice if the said evil
% space somehow managed to creep in.



% The paper headers
%\markboth{Journal of \LaTeX\ Class Files,~Vol.~6, No.~1, January~2007}%
%{Shell \MakeLowercase{\textit{et al.}}: Bare Demo of IEEEtran.cls for Journals}
% The only time the second header will appear is for the odd numbered pages
% after the title page when using the twoside option.
% 
% *** Note that you probably will NOT want to include the author's ***
% *** name in the headers of peer review papers.                   ***
% You can use \ifCLASSOPTIONpeerreview for conditional compilation here if
% you desire.




% If you want to put a publisher's ID mark on the page you can do it like
% this:
%\IEEEpubid{0000--0000/00\$00.00~\copyright~2007 IEEE}
% Remember, if you use this you must call \IEEEpubidadjcol in the second
% column for its text to clear the IEEEpubid mark.



% make the title area
\maketitle

%\newpage

\tableofcontents

%\renewcommand{\thefigure}{\thesection.\theenumi}
%\renewcommand{\thetable}{\thesection.\theenumi}

\renewcommand{\thefigure}{\theenumi}
\renewcommand{\thetable}{\theenumi}

%\renewcommand{\theequation}{\thesection}


\bigskip

\begin{abstract}
This manual provides a simple introduction to Fourier Series
\end{abstract}
\section{Periodic Function}
Let 
\begin{align}
	x(t) &= A_0\abs{\sin\brak{2\pi f_0 t}}
	\label{eq:10-orig-diff-def}
\end{align}
\begin{enumerate}[label=\thesection.\arabic*
,ref=\thesection.\theenumi]
\item Plot $x(t)$.\\
\solution 
\begin{lstlisting}
wget https://raw.githubusercontent.com/kumarsuraj151/EE3900/master/charger/codes/1.1.py

\end{lstlisting}
\begin{figure}[!ht]
	\centering
	\includegraphics[width=\columnwidth]{./figs/1.1}
	\caption{}
	%\label{fig:ckt}
\end{figure}
\item Show that $x(t)$ is periodic and find its period.
\solution 
    If a signal $x(t)$ is periodic then
    \begin{align}
    x(t+T)=x(t)
    \end{align}
    where $T$ is known as fundamental period.
    \indent Since $|sin\theta|$ function is periodic, x(t) is also periodic.
    \begin{align}
\text{Fundamental Period}=T=\frac{1}{2}\brak{\frac{2 \pi}{2 \pi f_0}}\\
\label{eq:ftp}
=\frac{1}{2f_0}
    \end{align}
\end{enumerate}
\section{Fourier Series}
Consider $A_0 =12$ and $f_0 = 50$ for all numerical calculations.
\begin{enumerate}[label=\thesection.\arabic*,ref=\thesection.\theenumi]
\item If
%\cite{proakis_dsp}
\begin{align}
	x(t) = \sum_{k = -\infty}^{\infty}c_ke^{\j2\pi kf_0 t}
\label{eq:one-Z-complex}
\end{align}
show that 
\begin{align}
	c_k = f_0\int_{-\frac{1}{2f_0}}^{\frac{1}{2f_0}}x(t)e^{-\j2\pi kf_0 t}\, dt
\label{eq:one-Z}
\end{align}
\solution 
    From \eqref{eq:one-Z-complex},
    \begin{align}
            x(t) = \sum_{k = -\infty}^{\infty}c_ke^{\j2\pi kf_0 t}
    \end{align}
    Mulitply $e^{-\j2\pi lf_0 t}$ on both sides
    \begin{align}
    x(t)e^{-\j2\pi lf_0 t}=\sum_{k = -\infty}^{\infty}c_ke^{\j2\pi kf_0 t}e^{-\j2\pi lf_0 t}
    \end{align}
    Integrate on both sides with respect to 't' between $-T$ to $T$ where T is fundamental time period of x(t).\\
    Using \eqref{eq:ftp},
    \begin{align}
    T=\frac{1}{2f_0}
    \end{align}
    \begin{align}
    \int_{-\frac{1}{2f_0}}^{\frac{1}{2f_0}}x(t)e^{-\j2\pi kf_0 t}\, dt=\int_{-\frac{1}{2f_0}}^{\frac{1}{2f_0}}\sum_{k = -\infty}^{\infty}c_ke^{\j2\pi \brak{k-l}f_0 t}\,dt\\
    =\sum_{k = -\infty}^{\infty}c_k\int_{-\frac{1}{2f_0}}^{\frac{1}{2f_0}}e^{\j2\pi \brak{k-l}f_0 t}\,dt
    \end{align}
    The above integral:
    \begin{align}
    \int_{-\frac{1}{2f_0}}^{\frac{1}{2f_0}}e^{\j2\pi \brak{k-l}f_0 t}\,dt=
          \begin{cases}
0 & k\neq l
\\
 \int_{-\frac{1}{2f_0}}^{\frac{1}{2f_0}}1\,dt& k=l
\end{cases}
    \end{align}
    \begin{align}
   \therefore \int_{-\frac{1}{2f_0}}^{\frac{1}{2f_0}}x(t)e^{-\j2\pi kf_0 t}\, dt &=\brak{\frac{1}{f_0}}c_k\\
  \therefore c_k = f_0\int_{-\frac{1}{2f_0}}^{\frac{1}{2f_0}}x(t)e^{-\j2\pi kf_0 t}\, dt
    \end{align}
	\item Find $c_k$ for 
	\eqref{eq:10-orig-diff-def}\\
	\solution
	$c_k$ can be calculated even simpler by using
	\begin{align}
	c_k = 2f_0\int_{0}^{\frac{1}{2f_0}}x(t)e^{- \j2 \pi kf_0 t}\, dt
	\end{align}
	$x(t)=A_0 \sin\brak{2 \pi f_0t}$ in 0 to $\frac{1}{2f_0}$ region.\\
Also,
	\begin{align}
	\label{eq:sin}
 \sin \theta  =\frac{e^{\j\theta}-e^{-\j \theta}}{2\j} 
  \end{align}
  Using \eqref{eq:sin},
  \begin{align}
  c_k &= 2f_0\int_{0}^{\frac{1}{2f_0}}A_0 \brak{\frac{e^{\j2\pi f_0t}-e^{-\j 2\pi f_0t}}{2\j}} e^{- \j2 \pi kf_0 t}\,dt\\
  &=A_0f_0\int_{0}^{\frac{1}{2f_0}} \brak{\frac{e^{\j2\pi\brak{1-k} f_0t}-e^{\j 2\pi\brak{-1-k} f_0t}}{\j}}\,dt\\
&=A_0f_0\sbrak{\frac{e^{\j2\pi\brak{1-k} f_0t}}{-2\pi \brak{1-k}f_0}\Big|_0^{\frac{1}{2f_0}} - \frac{e^{\j2\pi\brak{-1-k} f_0t}}{-2\pi \brak{-1-k}f_0}\Big|_0^{\frac{1}{2f_0}}}\\
&=A_0\sbrak{\frac{e^{j\pi\brak{1-k}}-1}{2\pi\brak{k-1}}-\frac{e^{-j\pi\brak{1+k}}-1}{2\pi\brak{k+1}}}
  \end{align}
  \begin{equation}
  \label{eq:ck}
 = \begin{cases}
\frac{2A_0}{\pi\brak{1-k^2}}&k=even
\\
0&k=odd
\end{cases}
  \end{equation}
\item Verify 
	\eqref{eq:10-orig-diff-def}
	using python.\\
	\solution
\begin{lstlisting}
wget https://raw.githubusercontent.com/kumarsuraj151/EE3900/master/charger/codes/1.1.py
\end{lstlisting}
\begin{figure}[!ht]
	\centering
	\includegraphics[width=\columnwidth]{./figs/2.3}
	\caption{}
	%\label{fig:ckt}
\end{figure}
	\item Show that 
\begin{align}
	x(t) = \sum_{k = 0}^{\infty}\brak{a_k\cos{\j2\pi kf_0 t}+b_k\sin{\j2\pi kf_0 t}}
\label{eq:one-Z-real}
\end{align}
and obtain the formulae for $a_k$ and $b_k$.
\solution
    Using \eqref{eq:one-Z-complex},
    \begin{align}
    x(t) = \sum_{k = -\infty}^{\infty}c_ke^{\j2\pi kf_0 t}
    \end{align}
    As,
    \begin{align}
    e^{\j2\pi kf_0 t}=\cos\brak{2\pi kf_0 t}+j\sin\brak{2\pi kf_0 t}
    \end{align}
    Substituting leads to
    \begin{align}
    x(t) &= \sum_{k = -\infty}^{\infty}c_k\sbrak{\cos\brak{2\pi kf_0 t}+j\sin\brak{2\pi kf_0 t}}\\
    \label{eq:2.4}
    &=\sum_{k = -\infty}^{\infty}c_k\cos\brak{2\pi kf_0 t}+jc_k\sin\brak{2\pi kf_0 t}  \\ 
    &\nonumber =\sum_{k = -\infty}^{-1}\sbrak{c_k\cos\brak{2\pi kf_0 t}+  jc_k\sin\brak{2\pi kf_0 t}} \\ 
    &  + c_0+\sum_{k = 1}^{\infty}\sbrak{c_k\cos\brak{2\pi kf_0 t}+jc_k\sin\brak{2\pi kf_0 t}}
  \end{align}
  \begin{align}
    &\nonumber =\sum_{k = 1}^{\infty}\sbrak{c_{-k}\cos\brak{2\pi kf_0 t}-jc_{-k}\sin\brak{2\pi kf_0 t}}\\
    & +c_0+ \sum_{k = 1}^{\infty}\sbrak{c_k\cos\brak{2\pi kf_0 t}+jc_k\sin\brak{2\pi kf_0 t}}\\
    &=c_0+\sum_{k = 1}^{\infty}\sbrak{\brak{c_k+c_{-k}}\cos\brak{2\pi kf_0 t}+j\brak{c_k-c_{-k}}\sin\brak{2\pi kf_0 t}}
    \end{align}
    Replacing $\brak{c_k+c_{-k}}\to a_k$ and $j\brak{c_k-c_{-k}} \to b_k$,
    \begin{align}
&=c_0+    \sum_{k = 1}^{\infty}\brak{a_k\cos{2\pi kf_0 t}+b_k\sin{2\pi kf_0 t}}\\
&=\sum_{k = 0}^{\infty}\brak{a_k\cos{2\pi kf_0 t}+b_k\sin{2\pi kf_0 t}}
    \end{align}
    \begin{align}
    \label{eq:u1}
    \therefore a_k=
    \begin{cases}
    c_k+c_{-k}&k\neq0
    \\
    c_0&k=0
    \end{cases}\\
    \label{eq:u2}
    b_k=j\brak{c_k-c_{-k}}
    \end{align}
    Using \eqref{eq:one-Z},
    \begin{align}
    c_k = f_0\int_{-\frac{1}{2f_0}}^{\frac{1}{2f_0}}x(t)e^{-\j2\pi kf_0 t}\, dt\\
    c_{-k} = f_0\int_{-\frac{1}{2f_0}}^{\frac{1}{2f_0}}x(t)e^{\j2\pi kf_0 t}\, dt\end{align}
    \begin{align}
    a_k=c_k+c_{-k}&= f_0\int_{-\frac{1}{2f_0}}^{\frac{1}{2f_0}}x(t)\sbrak{e^{-\j2\pi kf_0 t}+e^{\j2\pi kf_0 t}}\, dt\\
    &=2f_0\int_{-\frac{1}{2f_0}}^{\frac{1}{2f_0}}x(t)\cos\brak{2\pi kf_0t}\, dt
    \end{align}
    Parallely,
    \begin{align}
    b_k&=-2jf_0\int_{-\frac{1}{2f_0}}^{\frac{1}{2f_0}}x(t)\sin\brak{2\pi kf_0t}\, dt
    \end{align}
    \item Find $a_k$ and $b_k$ for 
        \eqref{eq:10-orig-diff-def}\\
        \solution
        Using \eqref{eq:u1} and \eqref{eq:u2} with \eqref{eq:ck},
    \begin{align}
    a_k=c_k+c_{-k}=\begin{cases}
\frac{4A_0}{\pi\brak{1-k^2}}&k=even
\\
\frac{2A_0}{\pi}&k=0
\\
0&k=odd
\end{cases}\\
b_k=j\brak{c_k-c_{-k}}=0
    \end{align}
\item Verify 
\eqref{eq:one-Z-real}
using python.\\
\solution 
  \begin{lstlisting}
  wget https://raw.githubusercontent.com/kumarsuraj151/EE3900/master/charger/codes/1.1.py
  \end{lstlisting}
    \begin{figure}[!ht]
\centering
\includegraphics[width=\columnwidth]{./figs/2.6}
\caption{}
			%\label{fig:ckt}
\end{figure}

\end{enumerate}
\section{Fourier Transform}

 

\begin{enumerate}[label=\thesection.\arabic*
,ref=\thesection.\theenumi]
\item 
	\begin{align}
		\delta(t)&=0, \quad t\neq0
\\
		\int_{-\infty}^{\infty}\delta(t) \, dt&= 1
	\end{align}
 \item The Fourier Transform of $g(t)$ is
 \begin{align}
 G(f)=\int_{-\infty}^{\infty}g(t)e^{-j2\pi ft}\,dt
 \end{align}
 \item Show that 
 \begin{align}
	 g(t-t_0)&\system{F}G(f)e^{-j2\pi ft_0}\\
 \end{align}
 \solution 
 \begin{align}
 \mathcal{F}\cbrak{g(t-t_0)}=\int_{-\infty}^{\infty}g(t-t_0)e^{-j2\pi ft}\,dt\\
 =e^{-j2\pi ft_0}\int_{-\infty}^{\infty}g(t-t_0)e^{-j2\pi f\brak{t-t_0}}\,dt\\
=G(f)e^{-j2\pi ft_0}
 \end{align}
 \item Show that 
 \begin{align}
	 G(t)&\system{F}g(-f)
 \end{align}
 \solution From the definition of Inverse Fourier Transform
 \begin{align}
 g(t)=\int_{-\infty}^{\infty}G(f)e^{j2\pi ft}\,df
 \end{align}
 Replace t $\to$ f,
 \begin{align}
  g(f)=\int_{-\infty}^{\infty}G(t)e^{j2\pi ft}\,dt
  \end{align}
  Replace f $\to$ -f,
  \begin{align}
   g(-f)=\int_{-\infty}^{\infty}G(t)e^{-j2\pi ft}\,dt\\
    =\mathcal{F}\cbrak{G(t)}
  \end{align}
  \begin{align}
  \therefore  G(t)&\system{F}g(-f)
  \label{eq:dual}
 \end{align}
 \item $\delta(t)\system{F}?$\\
 \solution
 \begin{align}
 \foutranin{\delta(t)}=\foutranfin{\delta(t)}\\
 =\int_{-\infty}^{\infty}\delta(t)\,dt\\
 \end{align}
 Since $e^{-j2\pi ft}=1$ for t=0 and remaining integrand is zero for t $\neq0$.
 \begin{align}
  =\int_{-\infty}^{\infty}\delta(t)\,dt\\
  =1
 \end{align}
 \item $e^{-j2\pi f_0t}\system{F}?$\\
 \solution 
 \begin{align}
 \foutranin{e^{-j2\pi f_0t}}=\int_{-\infty}^{\infty}1\cdot e^{-j2\pi\brak{f+f_0}t}\,dt\\
 =\int_{-\infty}^{\infty}\foutranin{\delta(t)} e^{-j2\pi\brak{f+f_0}t}\,dt
 \end{align}
 Using \eqref{eq:duality},
 \begin{align}
 \label{eq:eft}
 =\delta(-(f+f_0))=\delta(f+f_0)
 \end{align}
 \item $\cos(2\pi f_0t)\system{F}?$\\
 \solution
 \begin{align}
 \foutranin{\cos(2\pi f_0t)}=\foutranin{\frac{{e^{j2\pi f_0t}+e^{-j2\pi f_0t}}}{2}}
 \end{align}
 Using \eqref{eq:eft},
 \begin{align}
 =\frac{\delta(f+f_0)+\delta(f-f_0)}{2}
 \end{align}
 \item Find the Fourier Transform of $x(t)$ and plot it.  Verify using python.\\
 \solution
 \begin{align}
  \foutranin{x(t)}=\foutranin{\sum_{k = -\infty}^{\infty}c_ke^{\j2\pi kf_0 t}}\\
  X(f)=\sum_{k = -\infty}^{\infty}c_k\delta(f-kf_0)
  \end{align}
 \item Show that 
 \begin{align}
	 \rect{t} \system{F} \sinc{t}
 \end{align}
 Verify using python.\\
 \solution
 \begin{align}
  \foutranin{\rect{t}}=\foutranfin{\rect{t}}\\
  =\int_{-\frac{1}{2}}^{\frac{1}{2}}1\cdot e^{-j2\pi ft}\,dt\\
  =\frac{e^{-j2\pi ft}}{-j2\pi f}\Big |_{-\frac{1}{2}}^{\frac{1}{2}}\\
 \label{eq:rectf}
  =\sinc{t}
  \end{align}
 \item 
$	 \sinc{t}\system{F} ?$.  Verify using python.\\
\solution
Using \eqref{eq:rectf}, \eqref{eq:dual} and even property of rect function,
\begin{align}
\label{eq:sinc}
\sinc{t}\system{F}\rect{t}
\end{align}
\end{enumerate}
\section{Filter}
\begin{enumerate}[label=\thesection.\arabic*
,ref=\thesection.\theenumi]
\item Find $H(f)$ which transforms $x(t)$ to DC 5V.
\solution
\begin{figure}[!ht]
\centering
\begin{tikzpicture}
\tikzstyle{block} = [draw, shape=rectangle, minimum height=3em, minimum width=4em, node distance=2cm, line width=1pt]
\node at (-2.5,0) (input) {$x[t]$};
\node [block] (h) {$h[t]$};
\node at (2.5,0) (output) {$x[t]*h[t]$};
\begin{scope}[line width=1pt]
         \draw[->] (input) -- (h);
         \draw[->] (h) -- (output); 
    \end{scope}
\end{tikzpicture}
\end{figure}
\begin{figure}[!ht]
\centering
\begin{tikzpicture}
\tikzstyle{block} = [draw, shape=rectangle, minimum height=3em, minimum width=4em, node distance=2cm, line width=1pt]
\node at (-2.5,0) (input) {$X(f)$};
\node [block] (h) {$H(f)$};
\node at (2.5,0) (output) {$X(f)H(f)$};
\begin{scope}[line width=1pt]
         \draw[->] (input) -- (h);
         \draw[->] (h) -- (output); 
    \end{scope}
\end{tikzpicture}
\end{figure}
\begin{align}
X(f)H(f)=V_0\delta(f)
\end{align}
Above equation indicates that H(f) will pass X(f) for f=0.\\
\,$\therefore$ H(f) should be a low pass filter.
\begin{align}
|H(f)|=\frac{V_0}{\brak{\frac{2A_0}{\pi}}}=\frac{V_0\pi}{2A_0}\\
H(f)=\frac{V_0\pi}{2A_0} \hspace{10pt}in\hspace{8pt}-2f_0\leq f\leq 2f_0\\
\label{eq:hf}
H(f)=\frac{V_0\pi}{2A_0}\rect{\frac{f}{4f_0}}
\end{align}
\item Find $h(t)$.
\solution 
Using \eqref{eq:hf} and \eqref{eq:sinc},
\begin{align}
h(t)=\frac{2V_0\pi f_0}{A_0}\sinc{4f_0t}
\end{align}
\item Verify your result using  through convolution.
\end{enumerate}
\section{Filter Design}
\begin{enumerate}[label=\thesection.\arabic*
,ref=\thesection.\theenumi]
\item Design a Butterworth filter for $H(f)$.
\item Design a Chebyschev filter for $H(f)$.
\item Design a circuit for your Butterworth filter.
\item Design a circuit for your Chebyschev filter.
\end{enumerate}


\end{document}
